fix: integrateInput

LeanYjs/Algorithm/Insert/Basic.lean
@@ -5,6 +5,29 @@ import LeanYjs.Algorithm.Basic
 
 variable {A: Type} [DecidableEq A]
 
+structure IntegrateInput (A : Type) where
+  originId : Option YjsId
+  rightOriginId : Option YjsId
+  content : A
+  id : YjsId
+
+def IntegrateInput.toItem (input : IntegrateInput A) (arr : Array (YjsItem A)) : Except IntegrateError (YjsItem A) := do
+  let originPtr <- match input.originId with
+    | some id =>
+      match arr.find? (fun item => item.id = id) with
+      | some item => Except.ok (YjsPtr.itemPtr item)
+      | none => Except.error IntegrateError.error
+    | none => Except.ok YjsPtr.first
+
+  let rightOriginPtr <- match input.rightOriginId with
+    | some id =>
+      match arr.find? (fun item => item.id = id) with
+      | some item => Except.ok (YjsPtr.itemPtr item)
+      | none => Except.error IntegrateError.error
+    | none => Except.ok YjsPtr.last
+
+  return YjsItem.mk originPtr rightOriginPtr input.id input.content false
+
 def findPtrIdx (p : YjsPtr A) (arr : Array (YjsItem A)) : Except IntegrateError Int :=
   match p with
   | YjsPtr.itemPtr item =>
@@ -19,7 +42,7 @@ def getElemExcept (arr : Array (YjsItem A)) (idx : Nat) : Except IntegrateError 
   | some item => return item
   | none => Except.error IntegrateError.error
 
-def findIntegratedIndex (leftIdx rightIdx : Int) (newItem : YjsItem A) (arr : Array (YjsItem A)) : Except IntegrateError Nat := do
+def findIntegratedIndex (leftIdx rightIdx : Int) (newItem : IntegrateInput A) (arr : Array (YjsItem A)) : Except IntegrateError Nat := do
   let mut scanning := false
   let mut destIdx := leftIdx + 1
   for offset in [1:(rightIdx-leftIdx).toNat] do
@@ -44,18 +67,47 @@ def findIntegratedIndex (leftIdx rightIdx : Int) (newItem : YjsItem A) (arr : Ar
 
   return (Int.toNat destIdx)
 
-def integrate (newItem : YjsItem A) (arr : Array (YjsItem A)) : Except IntegrateError (Array (YjsItem A)) := do
-  let leftIdx <- findPtrIdx (YjsItem.origin newItem) arr
-  let rightIdx <- findPtrIdx (YjsItem.rightOrigin newItem) arr
+def findLeftIdx (originId : Option YjsId) (arr : Array (YjsItem A)) : Except IntegrateError Int :=
+  match originId with
+  | some id =>
+    match arr.findIdx? (fun item => item.id = id) with
+    | some idx => return idx
+    | none => Except.error IntegrateError.error
+  | none => return -1
 
+def findRightIdx (rightOriginId : Option YjsId) (arr : Array (YjsItem A)) : Except IntegrateError Int :=
+  match rightOriginId with
+  | some id =>
+    match arr.findFinIdx? (fun item => item.id = id) with
+    | some idx => return idx
+    | none => Except.error IntegrateError.error
+  | none => return arr.size
+
+def getPtrExcept (arr : Array (YjsItem A)) (idx : ℤ) : Except IntegrateError (YjsPtr A) :=
+  if idx = -1 then
+    Except.ok YjsPtr.first
+  else if idx = arr.size then
+    Except.ok YjsPtr.last
+  else
+    match arr[idx.toNat]? with
+    | some item => Except.ok (YjsPtr.itemPtr item)
+    | none => Except.error IntegrateError.error
+
+def mkItemByIndex (leftIdx rightIdx : Int) (input : IntegrateInput A) (arr : Array (YjsItem A)) : Except IntegrateError (YjsItem A) := do
+  return YjsItem.mk (← getPtrExcept arr leftIdx) (← getPtrExcept arr rightIdx) input.id input.content false
+
+def integrate (newItem : IntegrateInput A) (arr : Array (YjsItem A)) : Except IntegrateError (Array (YjsItem A)) := do
+  let leftIdx <- findLeftIdx newItem.originId arr
+  let rightIdx <- findRightIdx newItem.rightOriginId arr
   let destIdx <- findIntegratedIndex leftIdx rightIdx newItem arr
 
-  return (arr.insertIdxIfInBounds (Int.toNat destIdx) newItem)
+  let newItem := ← mkItemByIndex leftIdx rightIdx newItem arr
+  return arr.insertIdxIfInBounds (Int.toNat destIdx) newItem
 
-def isClockSafe (newItem : YjsItem A) (arr : Array (YjsItem A)) : Bool :=
+def isClockSafe (newItem : IntegrateInput A) (arr : Array (YjsItem A)) : Bool :=
   arr.all (fun item => item.id.clientId = newItem.id.clientId → newItem.id.clock > item.id.clock)
 
-def integrateSafe (newItem : YjsItem A) (arr : Array (YjsItem A)) : Except IntegrateError (Array (YjsItem A)) := do
+def integrateSafe (newItem : IntegrateInput A) (arr : Array (YjsItem A)) : Except IntegrateError (Array (YjsItem A)) := do
   if isClockSafe newItem arr then
     integrate newItem arr
   else
@@ -64,8 +116,8 @@ def integrateSafe (newItem : YjsItem A) (arr : Array (YjsItem A)) : Except Integ
 section Test
 
 def init : Array (YjsItem String)  := #[]
-def i1 := YjsItem.mk (YjsPtr.first) (YjsPtr.last) (YjsId.mk 0 0) "0" false
-def i2 := YjsItem.mk (YjsPtr.first) (YjsPtr.last) (YjsId.mk 0 1) "1" false
+def i1 := IntegrateInput.mk none none "0" (YjsId.mk 0 0)
+def i2 := IntegrateInput.mk none none "1" (YjsId.mk 0 1)
 
 def test12 := do
   let arr1 <- integrate i1 init
